Source/Core/Monomorphization.cs
@@ -246,34 +246,6 @@ namespace Microsoft.Boogie
   
   class ExprMonomorphizationVisitor : Duplicator
   {
-    private class TypeInstantiationComparer : IEqualityComparer<List<Type>>
-    {
-      public bool Equals(List<Type> l1, List<Type> l2)
-      {
-        if (l1.Count != l2.Count)
-        {
-          return false;
-        }
-
-        for (int i = 0; i < l1.Count; i++)
-        {
-          if (!l1[i].Equals(l2[i]))
-          {
-            return false;
-          }
-        }
-
-        return true;
-      }
-
-      public int GetHashCode(List<Type> l)
-      {
-        int hCode = 0;
-        l.Iter(x => { hCode = hCode ^ x.GetHashCode(); });
-        return hCode.GetHashCode();
-      }
-    }
-
     private Dictionary<Function, Dictionary<List<Type>, Function>> functionInstantiations;
     private Dictionary<DatatypeTypeCtorDecl, Dictionary<List<Type>, DatatypeTypeCtorDecl>> datatypeInstantiations;
     private Dictionary<TypeCtorDecl, HashSet<CtorType>> triggerTypes;
@@ -296,25 +268,8 @@ namespace Microsoft.Boogie
       variableMapping = new Dictionary<Variable, Variable>();
       boundVarSubst = new Dictionary<Variable, Variable>();
     }
-    
-    public static List<Axiom> InstantiateAxiom(
-      Dictionary<Function, Dictionary<List<Type>, Function>> functionInstantiations,
-      Dictionary<DatatypeTypeCtorDecl, Dictionary<List<Type>, DatatypeTypeCtorDecl>> datatypeInstantiations,
-      Dictionary<TypeCtorDecl, HashSet<CtorType>> triggerTypes,
-      Dictionary<TypeCtorDecl, HashSet<CtorType>> newTriggerTypes,
-      Axiom axiom,
-      HashSet<CtorType> triggers)
-    {
-      var instantiatedAxioms = new List<Axiom>();
-      var visitor = new ExprMonomorphizationVisitor(functionInstantiations, datatypeInstantiations, triggerTypes, newTriggerTypes);
-      triggers.Iter(trigger =>
-      {
-        instantiatedAxioms.Add(visitor.InstantiateAxiom(axiom, trigger.Arguments));
-      });
-      return instantiatedAxioms;
-    }
-    
-    private Axiom InstantiateAxiom(Axiom axiom, List<Type> funcTypeParamInstantiations)
+
+    public Axiom InstantiateAxiom(Axiom axiom, List<Type> funcTypeParamInstantiations)
     {
       var forallExpr = (ForallExpr) axiom.Expr;
       var savedTypeParamInstantiation = this.typeParamInstantiation;
@@ -325,12 +280,8 @@ namespace Microsoft.Boogie
       return new Axiom(axiom.tok, forallExpr.Dummies.Count == 0 ? forallExpr.Body : forallExpr, axiom.Comment, axiom.Attributes);
     }
     
-    private Function InstantiateFunction(Function func, List<Type> funcTypeParamInstantiations)
+    public Function InstantiateFunction(Function func, List<Type> funcTypeParamInstantiations)
     {
-      if (!functionInstantiations.ContainsKey(func))
-      {
-        functionInstantiations[func] = new Dictionary<List<Type>, Function>(new TypeInstantiationComparer());
-      }
       if (!functionInstantiations[func].ContainsKey(funcTypeParamInstantiations))
       {
         var funcTypeParamInstantiation = LinqExtender.Map(func.TypeParameters, funcTypeParamInstantiations);
@@ -393,14 +344,8 @@ namespace Microsoft.Boogie
       return instantiatedFunction;
     }
 
-    private void InstantiateDatatype(DatatypeTypeCtorDecl datatypeTypeCtorDecl,
-      List<Type> typeParamInstantiations)
+    private void InstantiateDatatype(DatatypeTypeCtorDecl datatypeTypeCtorDecl, List<Type> typeParamInstantiations)
     {
-      if (!datatypeInstantiations.ContainsKey(datatypeTypeCtorDecl))
-      {
-        datatypeInstantiations[datatypeTypeCtorDecl] =
-          new Dictionary<List<Type>, DatatypeTypeCtorDecl>(new TypeInstantiationComparer());
-      }
       if (!datatypeInstantiations[datatypeTypeCtorDecl].ContainsKey(typeParamInstantiations))
       {
         var newDatatypeTypeCtorDecl = new DatatypeTypeCtorDecl(
@@ -592,7 +537,7 @@ namespace Microsoft.Boogie
     }
   }
 
-  public class MonomorphizationVisitor : StandardVisitor
+  public class Monomorphizer : StandardVisitor
   {
     public static bool Monomorphize(Program program)
     {
@@ -600,41 +545,57 @@ namespace Microsoft.Boogie
       var isMonomorphizable = MonomorphizableChecker.IsMonomorphizable(program, out axiomsToBeInstantiated, out polymorphicFunctionAxioms);
       if (isMonomorphizable)
       {
-        var visitor = new MonomorphizationVisitor(program, axiomsToBeInstantiated, polymorphicFunctionAxioms);
-        visitor.VisitProgram(program);
-        visitor.InstantiateAxioms(axiomsToBeInstantiated);
-        program.RemoveTopLevelDeclarations(x => x is Function && ((Function) x).TypeParameters.Count > 0);
-        program.RemoveTopLevelDeclarations(x => axiomsToBeInstantiated.Contains(x) || polymorphicFunctionAxioms.Contains(x));
-        program.RemoveTopLevelDeclarations(x => x is DatatypeTypeCtorDecl y && y.Arity > 0);
-        visitor.functionInstantiations.Values.Iter(x =>
-        {
-          program.AddTopLevelDeclarations(x.Values);
-          x.Values.Where(y => y.DefinitionAxiom != null).Iter(y => program.AddTopLevelDeclaration(y.DefinitionAxiom));
-        });
-        program.AddTopLevelDeclarations(visitor.axiomInstantiations);
-        visitor.datatypeInstantiations.Values.Iter(x => program.AddTopLevelDeclarations(x.Values));
+        var monomorphizer = new Monomorphizer(program, axiomsToBeInstantiated, polymorphicFunctionAxioms);
+        monomorphizer.VisitProgram(program);
+        monomorphizer.InstantiateAxioms();
+        monomorphizer.UpdateInstantiatedDeclarations();
         Contract.Assert(PolymorphismChecker.IsMonomorphic(program));
+        program.monomorphizer = monomorphizer;
         return true;
       }
       return false;
     }
+
+    public Function Monomorphize(string functionName, Dictionary<string, Type> typeParamInstantiationMap)
+    {
+      if (!nameToFunction.ContainsKey(functionName))
+      {
+        return null;
+      }
+      var function = nameToFunction[functionName];
+      var typeParamInstantiations = function.TypeParameters.Select(tp => typeParamInstantiationMap[tp.Name]).ToList();
+      var instantiatedFunction = exprMonomorphizationVisitor.InstantiateFunction(function, typeParamInstantiations);
+      InstantiateAxioms();
+      UpdateInstantiatedDeclarations();
+      return instantiatedFunction;
+    }
     
     private Program program;
     private HashSet<Axiom> axiomsToBeInstantiated;
-    private HashSet<Axiom> polymorphicFunctionAxioms;
     private Dictionary<Function, Dictionary<List<Type>, Function>> functionInstantiations;
     private Dictionary<DatatypeTypeCtorDecl, Dictionary<List<Type>, DatatypeTypeCtorDecl>> datatypeInstantiations;
     private List<Axiom> axiomInstantiations;
     private Dictionary<TypeCtorDecl, HashSet<CtorType>> triggerTypes;
     private Dictionary<TypeCtorDecl, HashSet<CtorType>> newTriggerTypes;
+    private Dictionary<string, Function> nameToFunction;
+    private ExprMonomorphizationVisitor exprMonomorphizationVisitor;
+    private HashSet<Declaration> allInstantiatedDeclarations;
     
-    private MonomorphizationVisitor(Program program, HashSet<Axiom> axiomsToBeInstantiated, HashSet<Axiom> polymorphicFunctionAxioms)
+    private Monomorphizer(Program program, HashSet<Axiom> axiomsToBeInstantiated, HashSet<Axiom> polymorphicFunctionAxioms)
     {
       this.program = program;
       this.axiomsToBeInstantiated = axiomsToBeInstantiated;
-      this.polymorphicFunctionAxioms = polymorphicFunctionAxioms;
       functionInstantiations = new Dictionary<Function, Dictionary<List<Type>, Function>>();
+      nameToFunction = new Dictionary<string, Function>();
+      program.TopLevelDeclarations.OfType<Function>().Where(function => function.TypeParameters.Count > 0).Iter(
+        function =>
+        {
+          nameToFunction.Add(function.Name, function);
+          functionInstantiations.Add(function, new Dictionary<List<Type>, Function>(new TypeInstantiationComparer()));
+        });
       datatypeInstantiations = new Dictionary<DatatypeTypeCtorDecl, Dictionary<List<Type>, DatatypeTypeCtorDecl>>();
+      program.TopLevelDeclarations.OfType<DatatypeTypeCtorDecl>().Where(datatypeTypeCtorDecl => datatypeTypeCtorDecl.Arity > 0).Iter(datatypeTypeCtorDecl => 
+        datatypeInstantiations.Add(datatypeTypeCtorDecl, new Dictionary<List<Type>, DatatypeTypeCtorDecl>(new TypeInstantiationComparer())));
       axiomInstantiations = new List<Axiom>();
       triggerTypes = new Dictionary<TypeCtorDecl, HashSet<CtorType>>();
       newTriggerTypes = new Dictionary<TypeCtorDecl, HashSet<CtorType>>();
@@ -642,6 +603,48 @@ namespace Microsoft.Boogie
       {
         triggerTypes.Add(typeCtorDecl, new HashSet<CtorType>());
         newTriggerTypes.Add(typeCtorDecl, new HashSet<CtorType>());
+      });
+      exprMonomorphizationVisitor = new ExprMonomorphizationVisitor(functionInstantiations, datatypeInstantiations, triggerTypes, newTriggerTypes);
+      allInstantiatedDeclarations = new HashSet<Declaration>();
+      
+      program.RemoveTopLevelDeclarations(decl => 
+        decl is Function function && functionInstantiations.ContainsKey(function) ||
+        decl is DatatypeTypeCtorDecl datatypeTypeCtorDecl && datatypeInstantiations.ContainsKey(datatypeTypeCtorDecl) ||
+        axiomsToBeInstantiated.Contains(decl) || 
+        polymorphicFunctionAxioms.Contains(decl));
+    }
+
+    private void UpdateInstantiatedDeclarations()
+    {
+      functionInstantiations.Values.Iter(x =>
+        x.Values.Iter(function =>
+        {
+          if (!allInstantiatedDeclarations.Contains(function))
+          {
+            allInstantiatedDeclarations.Add(function);
+            program.AddTopLevelDeclaration(function);
+            if (function.DefinitionAxiom != null)
+            {
+              allInstantiatedDeclarations.Add(function.DefinitionAxiom);
+              program.AddTopLevelDeclaration(function.DefinitionAxiom);
+            }
+          }
+        }));
+      datatypeInstantiations.Values.Iter(x => x.Values.Iter(datatypeTypeCtorDecl =>
+      {
+        if (!allInstantiatedDeclarations.Contains(datatypeTypeCtorDecl))
+        {
+          allInstantiatedDeclarations.Add(datatypeTypeCtorDecl);
+          program.AddTopLevelDeclaration(datatypeTypeCtorDecl);
+        }
+      }));
+      axiomInstantiations.Iter(axiom =>
+      {
+        if (!allInstantiatedDeclarations.Contains(axiom))
+        {
+          allInstantiatedDeclarations.Add(axiom);
+          program.AddTopLevelDeclaration(axiom);
+        }
       });
     }
 
@@ -651,7 +654,7 @@ namespace Microsoft.Boogie
         .First(tcd => tcd.Name == axiom.FindStringAttribute("ctor"));
     }
 
-    private void InstantiateAxioms(HashSet<Axiom> axiomsToBeInstantiated)
+    private void InstantiateAxioms()
     {
       while (newTriggerTypes.Any(x => x.Value.Count != 0))
       {
@@ -660,41 +663,47 @@ namespace Microsoft.Boogie
         nextTriggerTypes.Iter(x => { newTriggerTypes.Add(x.Key, new HashSet<CtorType>()); });
         foreach (var axiom in axiomsToBeInstantiated)
         {
-          axiomInstantiations.AddRange(
-            ExprMonomorphizationVisitor.InstantiateAxiom(functionInstantiations, datatypeInstantiations,
-            triggerTypes, newTriggerTypes, axiom, nextTriggerTypes[GetTypeCtorDecl(axiom)]));
+          nextTriggerTypes[GetTypeCtorDecl(axiom)].Iter(trigger => axiomInstantiations.Add(exprMonomorphizationVisitor.InstantiateAxiom(axiom, trigger.Arguments)));
         }
       }
     }
 
     public override CtorType VisitCtorType(CtorType node)
     {
-      var exprVisitor = new ExprMonomorphizationVisitor(functionInstantiations, datatypeInstantiations, triggerTypes, newTriggerTypes);
-      return (CtorType) exprVisitor.VisitType(node);
+      return (CtorType) exprMonomorphizationVisitor.VisitType(node);
     }
     
     public override Expr VisitExpr(Expr node)
     {
-      var exprVisitor = new ExprMonomorphizationVisitor(functionInstantiations, datatypeInstantiations, triggerTypes, newTriggerTypes);
-      return exprVisitor.VisitExpr(node);
+      return exprMonomorphizationVisitor.VisitExpr(node);
     }
-
-    public override Function VisitFunction(Function node)
+    
+    private class TypeInstantiationComparer : IEqualityComparer<List<Type>>
     {
-      if (node.TypeParameters.Count > 0)
+      public bool Equals(List<Type> l1, List<Type> l2)
       {
-        return node;
-      }
-      return base.VisitFunction(node);
-    }
+        if (l1.Count != l2.Count)
+        {
+          return false;
+        }
 
-    public override Axiom VisitAxiom(Axiom node)
-    {
-      if (axiomsToBeInstantiated.Contains(node) || polymorphicFunctionAxioms.Contains(node))
-      {
-        return node;
+        for (int i = 0; i < l1.Count; i++)
+        {
+          if (!l1[i].Equals(l2[i]))
+          {
+            return false;
+          }
+        }
+
+        return true;
       }
-      return base.VisitAxiom(node);
+
+      public int GetHashCode(List<Type> l)
+      {
+        int hCode = 0;
+        l.Iter(x => { hCode = hCode ^ x.GetHashCode(); });
+        return hCode.GetHashCode();
+      }
     }
   }
 }
