Test/civl/linear/f2.bpl
@@ -1,26 +1,26 @@
-// RUN: %boogie -useArrayTheory -doModSetAnalysis "%s" > "%t"
+// RUN: %boogie -useArrayTheory -lib -monomorphize "%s" > "%t"
 // RUN: %diff "%s.expect" "%t"
-function {:builtin "MapConst"} mapconstbool(bool) : [int]bool;
-function {:builtin "MapOr"} mapunion([int]bool, [int]bool) : [int]bool;
 
-function {:inline} {:linear "1"} SetCollector1(x: [int]bool) : [int]bool
-{
-  x
-}
+
+
+
+
+
+type {:linear "1"} X = int;
 
 procedure Split({:linear_in "1"} xls: [int]bool) returns ({:linear "1"} xls1: [int]bool, {:linear "1"} xls2: [int]bool);
-ensures xls == mapunion(xls1, xls2) && xls1 != mapconstbool(false) && xls2 != mapconstbool(false);
+ensures xls == MapOr(xls1, xls2) && xls1 != MapConst(false) && xls2 != MapConst(false);
 
 procedure Allocate() returns ({:linear "1"} x: [int]bool);
 
-procedure main() 
+procedure main()
 {
    var {:linear "1"} x: [int] bool;
    var {:linear "1"} x1: [int] bool;
    var {:linear "1"} x2: [int] bool;
 
    call x := Allocate();
-   assume x == mapconstbool(true);
+   assume x == MapConst(true);
 
    call x1, x2 := Split(x);
    assert false;
