Test/civl/nocollector.bpl
@@ -1,7 +1,0 @@
-// RUN: %boogie -useArrayTheory "%s" > "%t"
-// RUN: %diff "%s.expect" "%t"
-var {:linear "L"} x:int;
-
-procedure{:yields}{:layer 1} P()
-{
-}
