Test/civl/signature-mismatch.bpl
@@ -1,6 +1,6 @@
-// RUN: %boogie -useArrayTheory "%s" > "%t"
+// RUN: %boogie -useArrayTheory -lib -monomorphize "%s" > "%t"
 // RUN: %diff "%s.expect" "%t"
-
+type {:linear "lin"} X = int;
 var {:layer 0,1} x:int;
 
 ////////////////////////////////////////////////////////////////////////////////
@@ -32,9 +32,3 @@ modifies x;
 { x := x'; }
 
 procedure {:yields} {:layer 0} {:refines "atomic_write_x_3"} write_x_3 ({:linear_in "lin"} x':int);
-
-function {:builtin "MapConst"} MapConstBool(bool) : [int]bool;
-function {:inline} {:linear "lin"} TidCollector(x: int) : [int]bool
-{
-  MapConstBool(false)[x := true]
-}
